\subsection*{Współrzędne biegunowe}
\begin{equation} \begin{cases}
    x = r \cos\varphi \\
    y = r \sin\varphi
\end{cases} \end{equation}
Jakobian przejścia to
\[ \det \frac{\p (x, y)}{\p (r, \varphi)} = \begin{vmatrix}
    \frac{\p x}{\p r} & \frac{\p x}{\p \varphi} \\
    \frac{\p y}{\p r} & \frac{\p y}{\p \varphi}
\end{vmatrix} = \begin{vmatrix}
    \cos\varphi & -r\sin\varphi \\
    \sin\varphi & r\cos\varphi
\end{vmatrix} = r\cos^2\varphi + r\sin^2\varphi = r. \]

\subsection*{Współrzędne walcowe}
\begin{equation} \begin{cases}
    x = r \cos\varphi \\
    y = r \sin\varphi \\
    z = z
\end{cases} \end{equation}
Jakobian przejścia to
\[ \det \frac{\p (x, y, z)}{\p (r, \varphi, z)} = \begin{vmatrix}
    \frac{\p x}{\p r} & \frac{\p x}{\p \varphi} & \frac{\p x}{\p z} \\
    \frac{\p y}{\p r} & \frac{\p y}{\p \varphi} & \frac{\p y}{\p z} \\
    \frac{\p z}{\p r} & \frac{\p z}{\p \varphi} & \frac{\p z}{\p z}
\end{vmatrix} = \begin{vmatrix}
    \cos\varphi & -r\sin\varphi & 0 \\
    \sin\varphi & r\cos\varphi & 0 \\
    0 & 0 & 1
\end{vmatrix} = r\cos^2\varphi + r\sin^2\varphi = r. \]

\subsection*{Współrzędne sferyczne}
\begin{equation} \begin{cases}
    x = r \cos\psi \cos\varphi \\
    y = r \cos\psi \sin\varphi \\
    z = r \sin\psi
\end{cases} \end{equation}
Jakobian przejścia to
\begin{align*}
    \det \frac{\p (x, y, z)}{\p (r, \psi, \varphi)} &= \begin{vmatrix}
        \frac{\p x}{\p r} & \frac{\p x}{\p \psi} & \frac{\p x}{\p \varphi} \\
        \frac{\p y}{\p r} & \frac{\p y}{\p \psi} & \frac{\p y}{\p \varphi} \\
        \frac{\p z}{\p r} & \frac{\p z}{\p \psi} & \frac{\p z}{\p \varphi}
    \end{vmatrix} = \begin{vmatrix}
        \cos\psi \cos\varphi & -r \sin\psi \cos\varphi & -r \cos\psi \sin\varphi \\
        \cos\psi \sin\varphi & -r \sin\psi \sin\varphi & r \cos\psi \cos\varphi \\
        \sin\psi & r \cos\psi & 0
    \end{vmatrix} \\
    &= r^2\cos\psi\left(-\sin^2\psi\cos^2\varphi - \cos^2\psi\sin^2\varphi - \sin^2\psi\sin^2\varphi - \cos^2\psi\cos^2\varphi\right) \\
    &= r^2\cos\psi\left(-\sin^2\psi - \cos^2\psi\right) \\
    &= -r^2\cos\psi.
\end{align*}
